adding exp to float types

src/lib/kuiper/Kuiper.Float32.fsti
@@ -3,8 +3,6 @@ module Kuiper.Float32
 new
 val t : Type0
 
-let float = t
-
 [@@noextract_to "krml"] val zero : t
 [@@noextract_to "krml"] val one : t
 
@@ -14,3 +12,7 @@ let float = t
 [@@noextract_to "krml"] val mul : t -> t -> t
 [@@noextract_to "krml"] val div : t -> t -> t
 [@@noextract_to "krml"] val rem : t -> t -> t
+
+[@@noextract_to "krml"] val exp : t -> t
+
+val add_comm (x y : t) : Lemma (add x y == add y x) [SMTPat (add x y)]
