src/lib/kuiper/Kuiper.Float64.fsti
@@ -3,8 +3,6 @@ module Kuiper.Float64
 new
 val t : Type0
 
-let double = t
-
 [@@noextract_to "krml"] val zero : t
 [@@noextract_to "krml"] val one : t
 
@@ -14,5 +12,7 @@ let double = t
 [@@noextract_to "krml"] val mul : t -> t -> t
 [@@noextract_to "krml"] val div : t -> t -> t
 [@@noextract_to "krml"] val rem : t -> t -> t
+
+[@@noextract_to "krml"] val exp : t -> t
 
 val add_comm (x y : t) : Lemma (add x y == add y x) [SMTPat (add x y)]
